\section*{6/3}
  \underline{Exercise 7.9}
    You have two machines. $M_1$ has lifetime $exp(\lambda_1)$ and $M_2$
    has lifetime $exp(\lambda_2)$. Let their lifetimes be $T_1$ and $T_2$.\\
    Machine 1 starts at time 0 and Machine 2 starts at time $t$.
    \begin{eqnarray*}
      P(\text{Machine 1 is the 1st to fail}) 
      & = & P(T_1 < T_2 + t)\\
      & = & P(T_1 < t)  + P(T_1 \ge t, T_1 < T_2 + t)\\
      & = & P(T_1 < t) + P(T_1 < T_2 + t |] T_1 \ge t) P(T_1 \ge t)\\
      & = & 1 - e^{-\lambda_1 t} + P(T_1 - t < T_2 | T_1 \ge t) e^{-\lambda_1 t}\\
      & = & 1 - e^{-\lambda_1 t} + P(T_1 < T_2) e^{-\lambda_1 t} \text{ (Memoryless probability.)}\\
      & = & 1 - e^{-\lambda_1 t} + \frac{\lambda_1}{\lambda_1 + \lambda_2} 
        e^{-\lambda_1 t} \text{ (Poisson process)}
    \end{eqnarray*}
    What if we replace $t$ with $T$, exponential (and independent of $T_1, T_2$)
    with parameter $\mu$?\\
    \begin{eqnarray*} 
      P(T_1 < T_2 + T)
      & = & P(T_1 < T) + P(T_1 \ge T, T_1 < T_2 + T)\\
      & = & \frac{\lambda_1}{\lambda_1 + \mu} + \frac{\lambda_1}{\lambda_1 + 
        \lambda_2}\frac{\mu}{\lambda_1 + \lambda_2}\\
    \end{eqnarray*}
  \underline{Example}: Hitchhiker's problem. You have $A$ and $B$. Cars that
  would pick up a hitchhiker approximately at a Poisson process at rate 
  $\lambda_0$. $A$ is first in line.\\
  After $exp(\lambda_A)$ time, $A$ quits.\\
  After $exp(\lambda_B)$ time, $B$ quits.\\
  \begin{eqnarray*}
    P(\text{A gets picked})
    & = & \frac{\lambda_{c}}{\lambda_{A} + \lambda_{c}}\\
    P(\text{B gets picked})
    & = & P(\text{at least 2 cars arrives before B quits} \bigcup \text{A quits
    and at least one car arrives before B quits})\\
    & = & P(\text{at least 2 cars arrives before B quits}) + P(\text{A quits
    and at least one car arrives before B quits}) - P(\text{A quits and at least
    2 cars arrive before B quits})\\
    & = & \left(\frac{\lambda_c}{\lambda_B + \lambda_c}\right)^2 + \left(
      \frac{\lambda_A}{\lambda_A + \lambda_B + \lambda_c}\right) \left(
      \frac{\lambda_c}{\lambda_A + \lambda_B + \lambda_c}\right) - \left(
      \frac{\lambda_A}{\lambda_A + \lambda_B + \lambda_c}\right) \left(
      \frac{\lambda_c}{\lambda_A + \lambda_B + \lambda_c}\right)^2\\
    & = & \frac{\lambda_A + \lambda_c}{\lambda_A + \lambda_B + \lambda_C} \cdot
      \frac{\lambda_C}{\lambda_B + \lambda_C}
  \end{eqnarray*}
  Better way:
  \begin{eqnarray*}
    P(\text{B gets picked})
    & = & P(\text{first event is either $A$ or $C$ and next event among $B$ and
      $C$ only has to be C})
  \end{eqnarray*}
